Big_Blue_Steps.thy
@@ -4,6 +4,185 @@ theory Big_Blue_Steps imports Book
 
 begin
 
+subsection \<open>Preliminaries: Fact D1\<close>
+
+text \<open>from appendix D, page 55\<close>
+lemma Fact_D1_73_aux:
+  fixes \<sigma>::real and m b::nat  
+  assumes \<sigma>: "0<\<sigma>" and bm: "real b < real m"
+  shows  "((\<sigma>*m) gchoose b) * inverse (m gchoose b) = \<sigma>^b * (\<Prod>i<b. 1 - ((1-\<sigma>)*i) / (\<sigma> * (real m - real i)))"
+proof -
+  have "((\<sigma>*m) gchoose b) * inverse (m gchoose b) = (\<Prod>i<b. (\<sigma>*m - i) / (real m - real i))"
+    using bm by (simp add: gbinomial_prod_rev prod_dividef atLeast0LessThan)
+  also have "\<dots> = \<sigma>^b * (\<Prod>i<b. 1 - ((1-\<sigma>)*i) / (\<sigma> * (real m - real i)))"
+    using bm
+  proof (induction b)
+    case 0
+    then show ?case
+      by simp
+  next
+    case (Suc b)
+    then have "b<m"
+      by linarith
+    with \<sigma> show ?case 
+      by (simp add: Suc field_simps)
+  qed
+  finally show ?thesis .
+qed
+
+text \<open>This is fact 4.2 (page 11) as well as equation (73), page 55.\<close>
+lemma Fact_D1_73:
+  fixes \<sigma>::real and m b::nat  
+  assumes \<sigma>: "0<\<sigma>" "\<sigma>\<le>1" and b: "real b \<le> \<sigma> * m / 2"
+  shows  "(\<sigma>*m) gchoose b \<in> {\<sigma>^b * (real m gchoose b) * exp (- (real b ^ 2) / (\<sigma>*m)) .. \<sigma>^b * (m gchoose b)}"
+proof (cases "m=0 \<or> b=0")
+  case True
+  then show ?thesis
+    using True assms by auto
+next
+  case False
+  then have "\<sigma> * m / 2 < real m"
+    using \<sigma> by auto
+  with b \<sigma> False have bm: "real b < real m"
+    by linarith
+  then have nonz: "m gchoose b \<noteq> 0"
+    by (simp add: flip: binomial_gbinomial)
+  have EQ: "((\<sigma>*m) gchoose b) * inverse (m gchoose b) = \<sigma>^b * (\<Prod>i<b. 1 - ((1-\<sigma>)*i) / (\<sigma> * (real m - real i)))" 
+    using Fact_D1_73_aux \<open>0<\<sigma>\<close> bm by blast
+  also have "\<dots> \<le> \<sigma> ^ b * 1"
+  proof (intro mult_left_mono prod_le_1 conjI)
+    fix i assume "i \<in> {..<b}"
+    with b \<sigma> bm show "0 \<le> 1 - (1 - \<sigma>) * i / (\<sigma> * (real m - i))"
+      by (simp add: field_split_simps)
+  qed (use \<sigma> bm in auto)
+  finally have upper: "(\<sigma>*m) gchoose b \<le> \<sigma>^b * (m gchoose b)"
+    using nonz by (simp add: divide_simps flip: binomial_gbinomial)
+  have *: "exp (-2 * real i / (\<sigma>*m)) \<le> 1 - ((1-\<sigma>)*i) / (\<sigma> * (real m - real i))" if "i<b" for i
+  proof -
+    have exp_le: "1-x \<ge> exp (-2 * x)" if "0 \<le>x" "x \<le> 1/2" for x::real
+    proof -
+      have "exp (-2 * x) = inverse (exp (2*x))"
+        by (simp add: exp_minus)
+      also have "\<dots> \<le> inverse (1 + 2*x)"
+        using exp_ge_add_one_self that by auto
+      also have "\<dots> \<le> 1-x"
+        using that by (simp add: mult_left_le field_simps)
+      finally show ?thesis .
+    qed
+    have "exp (-2 * real i / (\<sigma>*m)) = exp (-2 * (i / (\<sigma>*m)))"
+      by simp
+    also have "\<dots> \<le> 1 - i/(\<sigma> * m)"
+    using b that by (intro exp_le) auto
+    also have "\<dots> \<le> 1 - ((1-\<sigma>)*i) / (\<sigma> * (real m - real i))"
+      using \<sigma> b that 
+      apply (simp add: field_split_simps)
+      using bm by linarith
+    finally show ?thesis .
+  qed
+  have "sum real {..<b} \<le> real b ^ 2 / 2"
+    by (induction b) (auto simp: power2_eq_square algebra_simps)
+  with \<sigma> have "exp (- (real b ^ 2) / (\<sigma>*m)) \<le> exp (- (2 * (\<Sum>i<b. i) / (\<sigma>*m)))"
+    by (simp add: mult_less_0_iff divide_simps)
+  also have "\<dots> = exp (\<Sum>i<b. -2 * real i / (\<sigma>*m))"
+    by (simp add: sum_negf sum_distrib_left sum_divide_distrib)
+  also have "\<dots> = (\<Prod>i<b. exp (-2 * real i / (\<sigma>*m)))"
+    using exp_sum by blast
+  also have "\<dots> \<le> (\<Prod>i<b. 1 - ((1-\<sigma>)*i) / (\<sigma> * (real m - real i)))"
+    using * by (force intro: prod_mono)
+  finally have "exp (- (real b)\<^sup>2 / (\<sigma> * real m)) \<le> (\<Prod>i<b. 1 - (1 - \<sigma>) * real i / (\<sigma> * (real m - real i)))" .
+  with EQ have "\<sigma>^b * exp (- (real b ^ 2) / (\<sigma>*m)) \<le> ((\<sigma>*m) gchoose b) * inverse (real m gchoose b)"
+    by (simp add: \<sigma>)
+  with \<sigma> bm have lower: "\<sigma>^b * (real m gchoose b) * exp (- (real b ^ 2) / (\<sigma>*m)) \<le> (\<sigma>*m) gchoose b"
+    by (simp add: field_split_simps flip: binomial_gbinomial)
+  with upper show ?thesis 
+    by simp
+qed
+
+lemma exp_inequality_17:
+  fixes x::real
+  assumes "0 \<le> x" "x \<le> 1/7"
+  shows "1 - 4*x/3 \<ge> exp (-3*x/2)"
+proof -
+  have "x * 7 \<le> 1"
+    using assms by auto
+  with \<open>0 \<le> x\<close> have "45 * (x * (x * x)) + (42 * (x * x)) + 36/49 * x * x \<le> x * 8"
+    using assms by sos
+  moreover have "x * x * (36 * x * x) \<le> (1/7)*(1/7) * (36 * x * x)"
+    using assms by (intro mult_mono) auto
+  ultimately have *: "45 * (x * (x * x)) + (42 * (x * x) + x * (x * (x * x) * 36)) \<le> x * 8"
+    by simp
+  have "exp (-3*x/2) = inverse (exp (3*x/2))"
+    by (simp add: exp_minus)
+  also have "\<dots> \<le> inverse (1 + 3*x/2 + (1/2)*(3*x/2)^2 + (1/6)*(3*x/2)^3)"
+    apply (intro le_imp_inverse_le exp_lower_taylor_2)
+    by (smt (verit) divide_nonneg_nonneg mult_nonneg_nonneg \<open>0 \<le> x\<close> zero_le_power)
+  also have "\<dots> \<le> 1 - 4*x/3"
+    using assms *
+    apply (simp add: field_split_simps eval_nat_numeral not_less)
+    by (smt (verit, best) mult_nonneg_nonneg)
+  finally show ?thesis .
+qed
+
+text \<open>additional part\<close>
+lemma Fact_D1_75:
+  fixes \<sigma>::real and m b::nat  
+  assumes \<sigma>: "0<\<sigma>" "\<sigma><1" and b: "real b \<le> \<sigma> * m / 2" and b': "b \<le> m/7" and \<sigma>': "\<sigma> \<ge> 7/15"
+  shows  "(\<sigma>*m) gchoose b \<ge> exp (- (3 * real b ^ 2) / (4*m)) * \<sigma>^b * (m gchoose b)"
+proof (cases "m=0 \<or> b=0")
+  case True
+  then show ?thesis
+    using True assms by auto
+next
+  case False
+  with b \<sigma> have bm: "real b < real m"
+    by (smt (verit, ccfv_SIG) le_divide_eq_1_pos of_nat_le_0_iff pos_less_divide_eq times_divide_eq_left)
+  have *: "exp (- 3 * real i / (2*m)) \<le> 1 - ((1-\<sigma>)*i) / (\<sigma> * (real m - real i))" if "i<b" for i
+  proof -
+    have im: "0 \<le> i/m" "i/m \<le> 1/7"
+      using b' that by auto
+    have "exp (- 3* real i / (2*m)) \<le> 1 - 4*i / (3*m)"
+      using exp_inequality_17 [OF im] by (simp add: mult.commute)
+    also have "\<dots> \<le> 1 - 8*i / (7 * (real m - real b))"
+    proof -
+      have "real i * (real b * 7) \<le> real i * real m"
+        using b' by (simp add: mult_left_mono)
+      then show ?thesis
+        using b' by (simp add: field_split_simps)
+    qed
+    also have "\<dots> \<le> 1 - ((1-\<sigma>)*i) / (\<sigma> * (real m - real i))"
+    proof -
+      have 1: "(1 - \<sigma>) / \<sigma> \<le> 8/7"
+        using \<sigma> \<sigma>' that
+        by (simp add: field_split_simps)
+      have 2: "1 / (real m - real i) \<le> 1 / (real m - real b)"
+        using \<sigma> \<sigma>' b'  that by (simp add: field_split_simps)
+      have "(1 - \<sigma>) / (\<sigma> * (real m - real i)) \<le> 8 / (7 * (real m - real b))"
+        using mult_mono [OF 1 2] b' that by auto 
+      then show ?thesis
+        apply simp
+        by (metis mult.commute mult_left_mono of_nat_0_le_iff times_divide_eq_right)
+    qed
+    finally show ?thesis .
+  qed
+  have EQ: "((\<sigma>*m) gchoose b) * inverse (m gchoose b) = \<sigma>^b * (\<Prod>i<b. 1 - ((1-\<sigma>)*i) / (\<sigma> * (real m - real i)))" 
+    using Fact_D1_73_aux \<open>0<\<sigma>\<close> bm by blast
+  have "sum real {..<b} \<le> real b ^ 2 / 2"
+    by (induction b) (auto simp: power2_eq_square algebra_simps)
+  with \<sigma> have "exp (- (3 * real b ^ 2) / (4*m)) \<le> exp (- (3 * (\<Sum>i<b. i) / (2*m)))"
+    by (simp add: mult_less_0_iff divide_simps)
+  also have "\<dots> = exp (\<Sum>i<b. -3 * real i / (2*m))"
+    by (simp add: sum_negf sum_distrib_left sum_divide_distrib)
+  also have "\<dots> = (\<Prod>i<b. exp (-3 * real i / (2*m)))"
+    using exp_sum by blast
+  also have "\<dots> \<le> (\<Prod>i<b. 1 - ((1-\<sigma>)*i) / (\<sigma> * (real m - real i)))"
+    using * by (force intro: prod_mono)
+  finally have "exp (- (3 * real b ^ 2) / (4*m)) \<le> (\<Prod>i<b. 1 - (1-\<sigma>) * i / (\<sigma> * (real m - real i)))" .
+  with EQ have "\<sigma>^b * exp (- (3 * real b ^ 2) / (4*m)) \<le> ((\<sigma>*m) gchoose b) * inverse (m gchoose b)"
+    by (simp add: assms)
+  with \<sigma> bm show ?thesis
+    by (simp add: field_split_simps flip: binomial_gbinomial)
+qed
+
 lemma power2_12: "m \<ge> 12 \<Longrightarrow> 25 * m^2 \<le> 2^m"
 proof (induction m)
   case 0
